Generalize lvar type environments as stores

ContextStore/StoreFilterMapKey.v
@@ -1,7 +1,8 @@
 (** * Generic stores: partial key projection *)
 
-From ContextBase Require Import Prelude LogicVar.
+From ContextBase Require Import Prelude LogicVar LogicVarOpenEnv LogicVarShift.
 From ContextStore Require Import StoreCore StoreKeyAction.
+From ContextStore Require Import AtomEnv.
 
 Section StoreFilterMapKey.
 
@@ -38,5 +39,573 @@ Definition lvar_store_open (η : gmap nat atom) (s : LVarStore) : AtomStore :=
 
 Definition lvar_store_to_atom_store (s : LVarStore) : AtomStore :=
   lvar_store_open ∅ s.
+
+Definition lvar_store_shift_from (k : nat) (s : LVarStore) : LVarStore :=
+  storeA_rekey (logic_var_shift_from k) s.
+
+Definition lvar_store_shift (s : LVarStore) : LVarStore :=
+  lvar_store_shift_from 0 s.
+
+Definition lvar_store_open_one (k : nat) (x : atom)
+    (s : LVarStore) : LVarStore :=
+  storeA_rekey (logic_var_open k x) s.
+
+Definition lvar_store_open_lvars (η : gmap nat atom)
+    (s : LVarStore) : LVarStore :=
+  storeA_rekey (logic_var_open_env η) s.
+
+Definition lvar_store_atom_dom (s : LVarStore) : aset :=
+  lvars_fv (dom (s : gmap logic_var V)).
+
+Definition lvar_store_closed (s : LVarStore) : Prop :=
+  lvars_bv (dom (s : gmap logic_var V)) = ∅.
+
+Definition lvar_store_bvar_scope (s : LVarStore) : lvset :=
+  lvars_of_bvars (lvars_bv (dom (s : gmap logic_var V))).
+
+Definition lvar_store_swap (x y : atom) (s : LVarStore) : LVarStore :=
+  storeA_rekey (logic_var_swap x y) s.
+
+Lemma atom_store_to_lvar_store_dom (s : AtomStore) :
+  dom (atom_store_to_lvar_store s : gmap logic_var V) =
+  lvars_of_atoms (dom (s : gmap atom V)).
+Proof.
+  unfold atom_store_to_lvar_store, lvars_of_atoms.
+  apply storeA_map_key_dom.
+  intros x y Heq. inversion Heq. reflexivity.
+Qed.
+
+Lemma atom_store_to_lvar_store_insert x v (s : AtomStore) :
+  atom_store_to_lvar_store (<[x := v]> s) =
+  <[LVFree x := v]> (atom_store_to_lvar_store s).
+Proof.
+  unfold atom_store_to_lvar_store.
+  apply storeA_map_key_insert.
+  intros a b Heq. inversion Heq. reflexivity.
+Qed.
+
+Lemma atom_store_to_lvar_store_closed (s : AtomStore) :
+  lvar_store_closed (atom_store_to_lvar_store s).
+Proof.
+  unfold lvar_store_closed.
+  rewrite !atom_store_to_lvar_store_dom.
+  apply lvars_bv_of_atoms.
+Qed.
+
+Lemma atom_store_to_lvar_store_atom_dom (s : AtomStore) :
+  lvar_store_atom_dom (atom_store_to_lvar_store s) =
+  dom (s : gmap atom V).
+Proof.
+  unfold lvar_store_atom_dom.
+  rewrite atom_store_to_lvar_store_dom.
+  apply lvars_fv_of_atoms.
+Qed.
+
+Lemma atom_store_to_lvar_store_lookup_bound_none (s : AtomStore) k :
+  (atom_store_to_lvar_store s : gmap logic_var V) !! LVBound k = None.
+Proof.
+  apply not_elem_of_dom.
+  rewrite atom_store_to_lvar_store_dom.
+  unfold lvars_of_atoms.
+  intros Hin. apply elem_of_map in Hin as [x [Hbad _]].
+  discriminate.
+Qed.
+
+Lemma atom_store_to_lvar_store_lookup_free_none (s : AtomStore) x :
+  x ∉ dom (s : gmap atom V) ->
+  (atom_store_to_lvar_store s : gmap logic_var V) !! LVFree x = None.
+Proof.
+  intros Hfresh.
+  apply not_elem_of_dom.
+  rewrite atom_store_to_lvar_store_dom.
+  unfold lvars_of_atoms.
+  intros Hin. apply elem_of_map in Hin as [y [Hy HyD]].
+  inversion Hy. subst y. exact (Hfresh HyD).
+Qed.
+
+Lemma atom_store_to_lvar_store_lookup_free (s : AtomStore) x :
+  (atom_store_to_lvar_store s : gmap logic_var V) !! LVFree x =
+  (s : gmap atom V) !! x.
+Proof.
+  unfold atom_store_to_lvar_store.
+  change ((storeA_map_key LVFree s : gmap logic_var V) !! LVFree x =
+    (s : gmap atom V) !! x).
+  apply storeA_map_key_lookup.
+  intros a b Heq. inversion Heq. reflexivity.
+Qed.
+
+Lemma lvar_store_atom_dom_insert_bound (s : LVarStore) k v :
+  lvar_store_atom_dom (<[LVBound k := v]> s) = lvar_store_atom_dom s.
+Proof.
+  unfold lvar_store_atom_dom.
+  rewrite (dom_insert_L (M:=gmap logic_var) (D:=gset logic_var)
+    (s : gmap logic_var V) (LVBound k) v).
+  rewrite lvars_fv_union, lvars_fv_singleton_bound.
+  set_solver.
+Qed.
+
+Lemma logic_var_open_inj_fresh k x v1 v2 :
+  logic_var_open k x v1 = logic_var_open k x v2 ->
+  v1 = v2.
+Proof.
+  intros Heq.
+  rewrite <- (logic_var_open_involutive k x v1).
+  rewrite <- (logic_var_open_involutive k x v2).
+  by rewrite Heq.
+Qed.
+
+Lemma logic_var_open_inj k x :
+  Inj (=) (=) (logic_var_open k x).
+Proof.
+  intros v1 v2 Heq. eapply logic_var_open_inj_fresh. exact Heq.
+Qed.
+
+Lemma lvar_store_shift_free_notin_from k x (s : LVarStore) :
+  LVFree x ∉ dom (s : gmap logic_var V) ->
+  LVFree x ∉ dom (lvar_store_shift_from k s : gmap logic_var V).
+Proof.
+  intros Hfresh.
+  unfold lvar_store_shift_from.
+  change (LVFree x ∉ dom (storeA_rekey (logic_var_shift_from k) s : gmap logic_var V)).
+  rewrite storeA_rekey_dom by apply logic_var_shift_from_inj.
+  intros Hin. apply elem_of_map in Hin as [v [Hv HvD]].
+  destruct v as [n|y]; cbn [logic_var_shift_from] in Hv.
+  - destruct (decide (k <= n)); discriminate.
+  - inversion Hv. subst y. exact (Hfresh HvD).
+Qed.
+
+Lemma lvar_store_shift_free_notin x (s : LVarStore) :
+  LVFree x ∉ dom (s : gmap logic_var V) ->
+  LVFree x ∉ dom (lvar_store_shift s : gmap logic_var V).
+Proof.
+  apply lvar_store_shift_free_notin_from.
+Qed.
+
+Lemma lvar_store_shift_insert_from k v A (s : LVarStore) :
+  lvar_store_shift_from k (<[v := A]> s) =
+  <[logic_var_shift_from k v := A]> (lvar_store_shift_from k s).
+Proof.
+  unfold lvar_store_shift_from.
+  apply storeA_rekey_insert, logic_var_shift_from_inj.
+Qed.
+
+Lemma lvar_store_shift_insert v A (s : LVarStore) :
+  lvar_store_shift (<[v := A]> s) =
+  <[logic_var_shift_from 0 v := A]> (lvar_store_shift s).
+Proof.
+  apply lvar_store_shift_insert_from.
+Qed.
+
+Lemma lvar_store_shift_insert_free x A (s : LVarStore) :
+  lvar_store_shift (<[LVFree x := A]> s) =
+  <[LVFree x := A]> (lvar_store_shift s).
+Proof.
+  apply lvar_store_shift_insert.
+Qed.
+
+Lemma lvar_store_shift_atom_store (s : AtomStore) :
+  lvar_store_shift (atom_store_to_lvar_store s) = atom_store_to_lvar_store s.
+Proof.
+  apply storeA_map_eq. intros v.
+  destruct v as [k|x].
+  - transitivity (@None V).
+    + change (((lvar_store_shift (atom_store_to_lvar_store s) : LVarStore)
+          : gmap logic_var V) !! LVBound k = None).
+      apply not_elem_of_dom.
+      unfold lvar_store_shift, lvar_store_shift_from.
+      change (LVBound k ∉
+        dom (storeA_rekey (logic_var_shift_from 0) (atom_store_to_lvar_store s)
+          : gmap logic_var V)).
+      rewrite storeA_rekey_dom by apply logic_var_shift_from_inj.
+      intros Hin. apply elem_of_map in Hin as [u [Hu HuD]].
+      destruct u as [n|y]; cbn [logic_var_shift_from] in Hu.
+      * exfalso.
+        apply elem_of_dom in HuD as [A HA].
+        rewrite atom_store_to_lvar_store_lookup_bound_none in HA. discriminate.
+      * inversion Hu.
+    + symmetry. apply atom_store_to_lvar_store_lookup_bound_none.
+  - unfold lvar_store_shift, lvar_store_shift_from.
+    unfold storeA_rekey, storeA_map_key.
+    change ((kmap (M2:=gmap logic_var) (logic_var_shift_from 0)
+        (atom_store_to_lvar_store s)) !! LVFree x =
+      atom_store_to_lvar_store s !! LVFree x).
+    change (LVFree x) with (logic_var_shift_from 0 (LVFree x)) at 1.
+    rewrite (lookup_kmap (M1:=gmap logic_var) (M2:=gmap logic_var)
+      (Inj0:=logic_var_shift_from_inj 0)
+      (logic_var_shift_from 0) (atom_store_to_lvar_store s) (LVFree x)).
+    reflexivity.
+Qed.
+
+Lemma logic_var_swap_inj x y :
+  Inj (=) (=) (logic_var_swap x y).
+Proof.
+  intros v1 v2 Heq.
+  rewrite <- (logic_var_swap_involutive x y v1).
+  rewrite <- (logic_var_swap_involutive x y v2).
+  by rewrite Heq.
+Qed.
+
+Lemma logic_var_swap_match x y v :
+  match v with
+  | LVFree z => LVFree (swap x y z)
+  | LVBound k => LVBound k
+  end = logic_var_swap x y v.
+Proof.
+  destruct v as [k|z].
+  - rewrite logic_var_swap_unfold.
+    unfold swap. repeat destruct decide; congruence.
+  - rewrite logic_var_swap_unfold, logic_var_free_swap.
+    reflexivity.
+Qed.
+
+Lemma lvar_store_swap_lookup x y (s : LVarStore) v :
+  lvar_store_swap x y s !!
+    (match v with
+     | LVFree z => LVFree (swap x y z)
+     | LVBound k => LVBound k
+     end) = s !! v.
+Proof.
+  rewrite logic_var_swap_match.
+  unfold lvar_store_swap.
+  unfold storeA_rekey, storeA_map_key.
+  change ((kmap (M2:=gmap logic_var) (logic_var_swap x y) s) !!
+      logic_var_swap x y v = (s : gmap logic_var V) !! v).
+  rewrite (lookup_kmap (M1:=gmap logic_var) (M2:=gmap logic_var)
+    (Inj0:=logic_var_swap_inj x y)
+    (logic_var_swap x y) s v).
+  reflexivity.
+Qed.
+
+Lemma lvar_store_swap_lookup_inv x y (s : LVarStore) v :
+  lvar_store_swap x y s !! v =
+  s !! (match v with
+        | LVFree z => LVFree (swap x y z)
+        | LVBound k => LVBound k
+        end).
+Proof.
+  rewrite logic_var_swap_match.
+  rewrite <- (logic_var_swap_involutive x y v) at 1.
+  rewrite <- logic_var_swap_match.
+  apply lvar_store_swap_lookup.
+Qed.
+
+Lemma lvar_store_swap_dom x y (s : LVarStore) :
+  dom (lvar_store_swap x y s : gmap logic_var V) =
+  lvars_swap x y (dom (s : gmap logic_var V)).
+Proof.
+  unfold lvar_store_swap, lvars_swap.
+  change (dom (storeA_rekey (logic_var_swap x y) s : gmap logic_var V) =
+    set_swap (LVFree x) (LVFree y) (dom (s : gmap logic_var V))).
+  rewrite storeA_rekey_dom by apply logic_var_swap_inj.
+  unfold set_swap.
+  apply set_eq. intros v.
+  rewrite !elem_of_map.
+  split.
+  - intros [u [-> Hu]]. exists u. split; [|exact Hu].
+    rewrite logic_var_swap_unfold. reflexivity.
+  - intros [u [-> Hu]]. exists u. split; [|exact Hu].
+    rewrite <- logic_var_swap_unfold. reflexivity.
+Qed.
+
+Lemma lvar_store_swap_insert x y (s : LVarStore) v A :
+  lvar_store_swap x y (<[v := A]> s) =
+  <[match v with
+     | LVFree z => LVFree (swap x y z)
+     | LVBound k => LVBound k
+     end := A]> (lvar_store_swap x y s).
+Proof.
+  rewrite logic_var_swap_match.
+  unfold lvar_store_swap.
+  apply storeA_rekey_insert, logic_var_swap_inj.
+Qed.
+
+Lemma lvar_store_swap_atom_dom x y (s : LVarStore) :
+  lvar_store_atom_dom (lvar_store_swap x y s) =
+  set_swap x y (lvar_store_atom_dom s).
+Proof.
+  apply set_eq. intros z.
+  unfold lvar_store_atom_dom.
+  rewrite elem_of_set_swap, !lvars_fv_elem.
+  split.
+  - intros Hz.
+    change (LVFree z ∈ dom ((lvar_store_swap x y s : LVarStore)
+      : gmap logic_var V)) in Hz.
+    apply elem_of_dom in Hz as [A Hz].
+    rewrite lvar_store_swap_lookup_inv in Hz.
+    change (LVFree (swap x y z) ∈ dom (s : gmap logic_var V)).
+    apply elem_of_dom. exists A. exact Hz.
+  - intros Hz.
+    change (LVFree (swap x y z) ∈ dom (s : gmap logic_var V)) in Hz.
+    apply elem_of_dom in Hz as [A Hlookup].
+    change (LVFree z ∈ dom ((lvar_store_swap x y s : LVarStore)
+      : gmap logic_var V)).
+    apply elem_of_dom. exists A.
+    rewrite lvar_store_swap_lookup_inv.
+    exact Hlookup.
+Qed.
+
+Lemma lvar_store_atom_dom_lookup_free (s : LVarStore) x A :
+  s !! LVFree x = Some A ->
+  x ∈ lvar_store_atom_dom s.
+Proof.
+  intros Hlookup.
+  unfold lvar_store_atom_dom.
+  apply lvars_fv_elem.
+  change (LVFree x ∈ dom (s : gmap logic_var V)).
+  apply elem_of_dom. eexists. exact Hlookup.
+Qed.
+
+Lemma lvar_store_swap_fresh x y (s : LVarStore) :
+  x ∉ lvar_store_atom_dom s ->
+  y ∉ lvar_store_atom_dom s ->
+  lvar_store_swap x y s = s.
+Proof.
+  intros Hx Hy.
+  apply storeA_map_eq. intros v.
+  rewrite lvar_store_swap_lookup_inv.
+  destruct v as [k|z]; cbn.
+  - reflexivity.
+  - destruct (decide (z = x)) as [->|Hzx].
+    + rewrite swap_l.
+      destruct (s !! LVFree y) eqn:Hlooky.
+      * exfalso. apply Hy. eapply lvar_store_atom_dom_lookup_free. exact Hlooky.
+      * destruct (s !! LVFree x) eqn:Hlookx.
+        -- exfalso. apply Hx. eapply lvar_store_atom_dom_lookup_free. exact Hlookx.
+        -- symmetry. exact Hlookx.
+    + destruct (decide (z = y)) as [->|Hzy].
+      * rewrite swap_r.
+        destruct (s !! LVFree x) eqn:Hlookx.
+        -- exfalso. apply Hx. eapply lvar_store_atom_dom_lookup_free. exact Hlookx.
+        -- destruct (s !! LVFree y) eqn:Hlooky.
+           ++ exfalso. apply Hy. eapply lvar_store_atom_dom_lookup_free. exact Hlooky.
+           ++ symmetry. exact Hlooky.
+      * rewrite swap_fresh by congruence. reflexivity.
+Qed.
+
+Lemma lvar_store_open_atom_store η (s : AtomStore) :
+  lvar_store_open η (atom_store_to_lvar_store s) = s.
+Proof.
+  refine (fin_maps.map_fold_ind (M:=gmap atom)
+    (fun s => lvar_store_open η (atom_store_to_lvar_store s) = s) _ _ s).
+  - unfold lvar_store_open, atom_store_to_lvar_store,
+      storeA_filter_map_key, storeA_map_key.
+    rewrite kmap_empty. reflexivity.
+  - intros x v s' Hfresh Hfold IH.
+    rewrite atom_store_to_lvar_store_insert.
+    unfold lvar_store_open, storeA_filter_map_key at 1.
+    rewrite (map_fold_insert_L
+      (M:=gmap logic_var)
+      (fun w A acc =>
+        match lvar_to_atom η w with
+        | Some y => <[y:=A]> acc
+        | None => acc
+        end)
+      (∅ : gmap atom V) (LVFree x) v (atom_store_to_lvar_store s')).
+    + change (map_fold
+        (fun w A acc =>
+          match lvar_to_atom η w with
+          | Some y => <[y:=A]> acc
+          | None => acc
+          end) ∅ (atom_store_to_lvar_store s'))
+        with (lvar_store_open η (atom_store_to_lvar_store s')).
+      cbn [lvar_to_atom logic_var_to_atom].
+      rewrite IH. reflexivity.
+    + intros i j Ai Aj acc Hne Hi Hj.
+      destruct i as [ki|xi], j as [kj|xj];
+        cbn [lvar_to_atom logic_var_to_atom] in *; try reflexivity.
+      * rewrite lookup_insert_ne in Hi by congruence.
+        rewrite atom_store_to_lvar_store_lookup_bound_none in Hi. discriminate.
+      * rewrite lookup_insert_ne in Hi by congruence.
+        rewrite atom_store_to_lvar_store_lookup_bound_none in Hi. discriminate.
+      * rewrite lookup_insert_ne in Hj by congruence.
+        rewrite atom_store_to_lvar_store_lookup_bound_none in Hj. discriminate.
+      * apply insert_insert_ne. congruence.
+    + apply atom_store_to_lvar_store_lookup_free_none.
+      apply not_elem_of_dom. exact Hfresh.
+Qed.
+
+Lemma lvar_store_to_atom_store_atom_store (s : AtomStore) :
+  lvar_store_to_atom_store (atom_store_to_lvar_store s) = s.
+Proof.
+  unfold lvar_store_to_atom_store.
+  apply lvar_store_open_atom_store.
+Qed.
+
+Lemma lvar_store_to_atom_store_lookup_some (s : LVarStore) x v :
+  lvar_store_to_atom_store s !! x = Some v ->
+  s !! LVFree x = Some v.
+Proof.
+  unfold lvar_store_to_atom_store, lvar_store_open.
+  refine (fin_maps.map_fold_ind (M:=gmap logic_var)
+    (fun s => forall x v,
+      map_fold
+        (fun w A acc =>
+          match lvar_to_atom ∅ w with
+          | Some y => <[y:=A]> acc
+          | None => acc
+          end) ∅ s !! x = Some v ->
+      s !! LVFree x = Some v) _ _ s x v).
+  - intros a A Hlookup.
+    rewrite (map_fold_empty (K:=logic_var) (M:=gmap logic_var)) in Hlookup.
+    change ((∅ : gmap atom V) !! a = Some A) in Hlookup.
+    rewrite lookup_empty in Hlookup. discriminate.
+  - intros w A s' Hfresh Hfold IH a B.
+    rewrite Hfold.
+    destruct w as [k|y]; cbn [lvar_to_atom logic_var_to_atom].
+    + intros Hlookup.
+      change ((<[LVBound k := A]> (s' : gmap logic_var V) :
+        gmap logic_var V) !! LVFree a = Some B).
+      rewrite (lookup_insert_ne (M:=gmap logic_var)) by discriminate.
+      apply IH. exact Hlookup.
+    + intros Hlookup.
+      apply (proj1 (lookup_insert_Some (M:=gmap atom)
+        (map_fold
+           (fun w A acc =>
+             match lvar_to_atom ∅ w with
+             | Some y => <[y:=A]> acc
+             | None => acc
+             end) ∅ s') y a A B)) in Hlookup.
+      destruct Hlookup as [[-> ->]|[Hya Hlookup]].
+      * change ((<[LVFree a := B]> (s' : gmap logic_var V) :
+          gmap logic_var V) !! LVFree a = Some B).
+        rewrite lookup_insert_eq. reflexivity.
+      * change ((<[LVFree y := A]> (s' : gmap logic_var V) :
+          gmap logic_var V) !! LVFree a = Some B).
+        rewrite (lookup_insert_ne (M:=gmap logic_var)) by congruence.
+        apply IH. exact Hlookup.
+Qed.
+
+Lemma lvar_store_to_atom_store_lookup_free_some (s : LVarStore) x v :
+  (s : gmap logic_var V) !! LVFree x = Some v ->
+  lvar_store_to_atom_store s !! x = Some v.
+Proof.
+  unfold lvar_store_to_atom_store, lvar_store_open.
+  refine (fin_maps.map_fold_ind (M:=gmap logic_var)
+    (fun s => forall x v,
+      (s : gmap logic_var V) !! LVFree x = Some v ->
+      map_fold
+        (fun w A acc =>
+          match lvar_to_atom ∅ w with
+          | Some y => <[y:=A]> acc
+          | None => acc
+          end) ∅ s !! x = Some v) _ _ s x v).
+  - intros a A Hlookup.
+    change ((∅ : gmap logic_var V) !! LVFree a = Some A) in Hlookup.
+    rewrite lookup_empty in Hlookup. discriminate.
+  - intros w A s' Hfresh Hfold IH a B Hlookup.
+    destruct w as [k|y]; cbn [lvar_to_atom logic_var_to_atom].
+    + rewrite Hfold.
+      change ((<[LVBound k := A]> (s' : gmap logic_var V) :
+        gmap logic_var V) !! LVFree a = Some B) in Hlookup.
+      rewrite (lookup_insert_ne (M:=gmap logic_var)) in Hlookup by discriminate.
+      apply IH. exact Hlookup.
+    + rewrite Hfold.
+      change ((<[LVFree y := A]> (s' : gmap logic_var V) :
+        gmap logic_var V) !! LVFree a = Some B) in Hlookup.
+      destruct (decide (y = a)) as [->|Hya].
+      * rewrite (lookup_insert_eq (M:=gmap logic_var)) in Hlookup.
+        inversion Hlookup. subst A.
+        cbn [lvar_to_atom logic_var_to_atom].
+        change (((<[a:=B]>
+          (map_fold
+             (fun w A acc =>
+               match lvar_to_atom ∅ w with
+               | Some y => <[y:=A]> acc
+               | None => acc
+               end) ∅ s' : gmap atom V)) : gmap atom V) !! a = Some B).
+        exact (lookup_insert_eq
+          (M:=gmap atom)
+          (map_fold
+             (fun w A acc =>
+               match lvar_to_atom ∅ w with
+               | Some y => <[y:=A]> acc
+               | None => acc
+               end) ∅ s' : gmap atom V) a B).
+      * rewrite (lookup_insert_ne (M:=gmap logic_var)) in Hlookup by congruence.
+        cbn [lvar_to_atom logic_var_to_atom].
+        change (((<[y:=A]>
+          (map_fold
+             (fun w A acc =>
+               match lvar_to_atom ∅ w with
+               | Some y => <[y:=A]> acc
+               | None => acc
+               end) ∅ s' : gmap atom V)) : gmap atom V) !! a = Some B).
+        replace (((<[y:=A]>
+          (map_fold
+             (fun w A acc =>
+               match lvar_to_atom ∅ w with
+               | Some y => <[y:=A]> acc
+               | None => acc
+               end) ∅ s' : gmap atom V)) : gmap atom V) !! a)
+          with ((map_fold
+             (fun w A acc =>
+               match lvar_to_atom ∅ w with
+               | Some y => <[y:=A]> acc
+               | None => acc
+               end) ∅ s' : gmap atom V) !! a).
+        -- apply IH. exact Hlookup.
+        -- symmetry. apply lookup_insert_ne. congruence.
+Qed.
+
+Lemma lvar_store_to_atom_store_lookup (s : LVarStore) x :
+  lvar_store_to_atom_store s !! x = (s : gmap logic_var V) !! LVFree x.
+Proof.
+  destruct (lvar_store_to_atom_store s !! x) as [v|] eqn:Hatom.
+  - apply lvar_store_to_atom_store_lookup_some in Hatom.
+    symmetry. exact Hatom.
+  - destruct ((s : gmap logic_var V) !! LVFree x) as [v|] eqn:Hlv;
+      [|reflexivity].
+    pose proof (lvar_store_to_atom_store_lookup_free_some s x v Hlv) as Hatom'.
+    rewrite Hatom in Hatom'. discriminate.
+Qed.
+
+Lemma lvar_store_to_atom_store_insert_free (s : LVarStore) x v :
+  lvar_store_to_atom_store (<[LVFree x := v]> s) =
+  <[x := v]> (lvar_store_to_atom_store s).
+Proof.
+  apply (map_eq (M:=gmap atom)). intros y.
+  rewrite lvar_store_to_atom_store_lookup.
+  destruct (decide (y = x)) as [->|Hyx].
+  - change ((((<[LVFree x := v]> (s : gmap logic_var V))
+        : gmap logic_var V) !! LVFree x) =
+      (((<[x := v]> (lvar_store_to_atom_store s)) : gmap atom V) !! x)).
+    rewrite (lookup_insert_eq (M:=gmap logic_var)).
+    change (Some v =
+      (((<[x := v]> (lvar_store_to_atom_store s)) : gmap atom V) !! x)).
+    symmetry.
+    exact (lookup_insert_eq (M:=gmap atom) (lvar_store_to_atom_store s) x v).
+  - rewrite (lookup_insert_ne (M:=gmap logic_var) (s : gmap logic_var V) (LVFree x) (LVFree y) v)
+      by congruence.
+    change ((s : gmap logic_var V) !! LVFree y =
+      (((<[x := v]> (lvar_store_to_atom_store s)) : gmap atom V) !! y)).
+    transitivity (lvar_store_to_atom_store s !! y).
+    + symmetry. apply lvar_store_to_atom_store_lookup.
+    + symmetry.
+      apply (lookup_insert_ne (M:=gmap atom)). congruence.
+Qed.
+
+Lemma lvar_store_to_atom_store_swap x y (s : LVarStore) :
+  lvar_store_to_atom_store (lvar_store_swap x y s) =
+  (kmap (swap x y) (lvar_store_to_atom_store s) : gmap atom V).
+Proof.
+  apply (map_eq (M:=gmap atom)). intros z.
+  rewrite lvar_store_to_atom_store_lookup.
+  transitivity (lvar_store_to_atom_store s !! swap x y z).
+  - rewrite lvar_store_swap_lookup_inv.
+    symmetry. apply lvar_store_to_atom_store_lookup.
+  - symmetry. apply kmap_swap_lookup_inv.
+Qed.
+
+Lemma lvar_store_to_atom_store_dom_subset (s : LVarStore) :
+  dom (lvar_store_to_atom_store s) ⊆ lvar_store_atom_dom s.
+Proof.
+  intros x Hx.
+  change (x ∈ dom (lvar_store_to_atom_store s : gmap atom V)) in Hx.
+  apply elem_of_dom in Hx as [v Hv].
+  apply lvar_store_to_atom_store_lookup_some in Hv.
+  unfold lvar_store_atom_dom.
+  apply lvars_fv_elem.
+  eapply storeA_elem_of_dom_lookup_some. exact Hv.
+Qed.
 
 End StoreFilterMapKey.
